...

bf/bf.thy
@@ -11,17 +11,62 @@ autocorres [
   (*no_signed_word_abs=init,*)
   unsigned_word_abs=init] "bf.c"
 
+term hrs_mem_update
+term t_hrs_'_update
+term heap_update_list
+term globals.a_'
+term globals.a_'
+thm globals.a_'_def
+term ptr_val
+term Arrays.update
+find_consts "'a['b]"
+
+fun aupda :: "8 word['b::finite] \<Rightarrow> nat \<Rightarrow> 8 word['b]" where
+  "aupda a 0 = Arrays.update a 0 0" |
+  "aupda a (Suc i) = aupda (Arrays.update a (Suc i) 0) i"
+
+lemma "i \<ge> CARD('b) \<Longrightarrow> aupda s i = Arrays.FCP (\<lambda>_. 0)"
+  apply(induction s i rule: aupda.induct)
+   apply(simp add: FCP_def Arrays.update_def)
+   
+  apply(simp)
+  apply(case_tac "i = 255")
+   apply(simp_all)
+  
+  oops
+  
+
+
+fun gaupda :: "globals \<Rightarrow> nat \<Rightarrow> globals" where
+  "gaupda s 0 = s\<lparr>globals.a_' := Arrays.update (globals.a_' s) 0 0\<rparr>" |
+  "gaupda s (Suc i) = gaupda (s\<lparr>globals.a_' := Arrays.update (globals.a_' s) i 0\<rparr>) i"
+
+
+lemma "i \<ge> CARD(256) \<Longrightarrow> gaupda s i = s\<lparr>globals.a_' := Arrays.FCP (\<lambda>_. 0)\<rparr>"
+  apply(induction s i rule: gaupda.induct)
+   apply(simp)
+  apply(simp)
+  apply(case_tac "i = 255")
+   apply(simp_all)
+  
+  oops
+  
+
 lemma (in bf) init:
   "\<forall>s\<^sub>0. \<lbrace> \<lambda>s.  s = s\<^sub>0 \<rbrace>
       init'
-        \<lbrace> \<lambda>rs s. s = t_hrs_'_update (hrs_mem_update (
-          heap_update_list (ptr_val p) (replicate 256 0))) s\<^sub>0  \<rbrace>!"
+        \<lbrace> \<lambda>rs s. s = s\<^sub>0\<lparr>globals.a_' := Arrays.FCP (\<lambda>_. 0)\<rparr>  \<rbrace>!"
+(*\<lbrace> \<lambda>rs s. s = t_hrs_'_update (hrs_mem_update (heap_update_list (addr) (replicate 255 0))) s\<^sub>0  \<rbrace>!*)
   unfolding init'_def
   apply(rule allI)
-  apply (subst whileLoop_add_inv[where I="\<lambda>i s. i \<le> 256 \<and> i \<ge> 0" and M="\<lambda>(i, _). nat (256 - i)"])
+  apply (subst whileLoop_add_inv[where I="\<lambda>i s. i \<le> 256 \<and> i \<ge> 0 \<and> s = gaupda s\<^sub>0 ((unat (of_int i)))" and M="\<lambda>(i, _). nat (256 - i)"])
   apply(wp)
   apply(simp_all)
   apply(simp add: INT_MAX_def)
+  
+  apply(clarsimp)
+  apply (clarsimp simp: FCP_def)
+  
   oops
   
 
